code/experimental/P256/Hacl.Impl.ECDSA.P256SHA256.Verification.fst
@@ -11,6 +11,7 @@ open Hacl.Spec.P256.Definitions
 open Hacl.Impl.LowLevel
 open Hacl.Impl.P256
 open Hacl.Spec.P256.MontgomeryMultiplication
+open Hacl.Impl.MM.Exponent
 
 val isCoordinateValid: p: lbuffer uint64 (size 12) -> Stack bool 
   (requires fun h -> live h p)
@@ -27,9 +28,9 @@ let isCoordinateValid p =
     let x = sub p (size 0) (size 4) in 
     let y = sub p (size 4) (size 4) in 
     let z = sub p (size 8) (size 4) in 
-    let carryX = sub4_il x prime_buffer tempBuffer in 
-    let carryY = sub4_il y prime_buffer tempBuffer in 
-    let carryZ = sub4_il z prime_buffer tempBuffer in 
+    let carryX = sub4_il x prime256_buffer tempBuffer in 
+    let carryY = sub4_il y prime256_buffer tempBuffer in 
+    let carryZ = sub4_il z prime256_buffer tempBuffer in 
 
     let lessX = eq #U64  carryX (u64 0) in 
     let lessY = eq #U64 carryY (u64 0) in 
@@ -38,16 +39,24 @@ let isCoordinateValid p =
       pop_frame()  ; 
     lessX && lessY && lessZ
 
-val computeInverse: a: felem -> b: felem -> Stack unit
-  (requires fun h -> True)
-  (ensures fun h0 _ h1 -> True)
 
-let computeInverse a b = 
-  push_frame();
-    let temp = create (size 20) (u64 0) in 
-    clean_exponent a b temp;
- pop_frame()   
-    
+
+val isOrderCorrect: p: lbuffer uint64 (size 12) -> tempBuffer: lbuffer uint64 (size 100) ->  Stack bool
+  (requires fun h -> live h p)
+  (ensures fun h0 _ h1 -> h0 == h1)
+
+let isOrderCorrect p tempBuffer= 
+  push_frame(); 
+    let order = create (size 32) (u8 0) in 
+    let multResult = create (size 4) (u64 0) in 
+    upload_scalar order;
+    scalarMultiplication p multResult order tempBuffer;
+    let result = isPointAtInfinity multResult in 
+ pop_frame();
+   result
+  
+
+
 
 
 val ecdsa_verification: 
@@ -63,10 +72,14 @@ val ecdsa_verification:
 
 
 let ecdsa_verification pubKey r s mLen m tempBuffer = 
+  push_frame();
+    let tempBuffer = create (size 100) (u64 0) in 
     (*check that publicKey is not equal to the identity element O *)
   (*let pointInfinityPublicKey = isPointAtInfinity pubKey in 
     if pointInfinityPublicKey = true then false else *)
   let coordinatesValid = isCoordinateValid pubKey in
     if coordinatesValid = true then false else 
   let belongsToCurve =  isPointOnCurve pubKey in 
-    if belongsToCurve = false then false else true
+    if belongsToCurve = false then false else 
+  let orderCorrect = isOrderCorrect pubKey tempBuffer in 
+    if orderCorrect = false then false else true
